tools/Vale/test/Vale.fst
@@ -130,9 +130,10 @@ let va_lemma_ifElse (ifb:ocmp) (ct:code) (cf:code) (s_0:va_state) (sN:va_state)
   = eval_ocmp s_0 ifb, s_0
 
 let va_whileInv (b:ocmp) (c:code{While? c}) (inv:operand) (s_0:va_state) (sN:va_state) =
-  eval_operand inv s_0 >= 0           /\
+  let open FStar.UInt64 in
+  (v (eval_operand inv s_0) >= 0           /\
   (forall (r:reg). s_0.regs `contains` r) /\
-  Some(sN) == eval_while c s_0
+  Some(sN) == eval_while c s_0)
 
 let va_lemma_while (b:ocmp) (c:code) (inv:operand) (s_0:va_state) (sN:va_state)
   :Pure va_state
@@ -140,9 +141,11 @@ let va_lemma_while (b:ocmp) (c:code) (inv:operand) (s_0:va_state) (sN:va_state)
 	(ensures  (fun s_1 -> Some(sN) == eval_while (While b c inv) s_0 /\ s_1 == s_0))
   = s_0
 
+open FStar.UInt64
+
 let va_lemma_whileTrue (b:ocmp) (c:code) (inv:operand) (s_0:va_state) (sN:va_state)
   :Pure (va_state * va_state)
-        (requires (eval_operand inv s_0 > 0 /\
+        (requires (v (eval_operand inv s_0) > 0 /\
 	           Some(sN) == eval_while (While b c inv) s_0))
 	(ensures  (fun (s_0', s_1) -> s_0' == s_0         /\
 	                          eval_ocmp s_0 b      /\
@@ -151,7 +154,7 @@ let va_lemma_whileTrue (b:ocmp) (c:code) (inv:operand) (s_0:va_state) (sN:va_sta
   = s_0, Some?.v (eval_code c s_0)
 
 let va_lemma_whileFalse (b:ocmp) (c:code) (inv:operand) (s_0:va_state) (sN:va_state)
-  :Pure va_state (requires (eval_operand inv s_0 == 0 /\
+  :Pure va_state (requires (eval_operand inv s_0 == 0uL /\
                             Some(sN) == eval_while (While b c inv) s_0))
 		 (ensures  (fun s_1 -> s_0 == s_1 /\ s_1 == sN /\ not (eval_ocmp s_0 b)))
   = s_0
